fix build, added TODOs for equiv

ArkLib/OracleReduction/Equiv.lean
@@ -50,10 +50,12 @@ section Relation
 
 variable {Stmt Wit Stmt' Wit' : Type}
 
-def Relation.equiv (f : Stmt ≃ Stmt') (g : Wit ≃ Wit') (R : Stmt → Wit → Prop) (R' : Stmt' → Wit' → Prop) : Prop :=
+def Relation.equiv (f : Stmt ≃ Stmt') (g : Wit ≃ Wit')
+    (R : Stmt → Wit → Prop) (R' : Stmt' → Wit' → Prop) : Prop :=
   ∀ stmt : Stmt, ∀ wit : Wit, R stmt wit ↔ R' (f stmt) (g wit)
 
-theorem Relation.equiv_symm (f : Stmt ≃ Stmt') (g : Wit ≃ Wit') (R : Stmt → Wit → Prop) (R' : Stmt' → Wit' → Prop) :
+theorem Relation.equiv_symm (f : Stmt ≃ Stmt') (g : Wit ≃ Wit')
+    (R : Stmt → Wit → Prop) (R' : Stmt' → Wit' → Prop) :
   Relation.equiv f g R R' ↔ Relation.equiv f.symm g.symm R' R := by
   simp [Relation.equiv]
   constructor
@@ -64,27 +66,72 @@ theorem Relation.equiv_symm (f : Stmt ≃ Stmt') (g : Wit ≃ Wit') (R : Stmt �
     intro stmt wit
     simpa using (h (f stmt) (g wit)).symm
 
--- TODO: define quotienting (i.e. statement is a product type and relation only depends on one component)
-
 end Relation
+
+namespace ProtocolSpec
+
+#check Equiv.instEquivLike
+
+/-- Two protocol specifications are equivalent if they have the same number of rounds, same
+  direction for each round, and an equivalence of types for each round. -/
+@[ext]
+structure Equiv {m n : ℕ} (pSpec : ProtocolSpec m) (pSpec' : ProtocolSpec n) where
+  round_eq : m = n
+  dir_eq : ∀ i, (pSpec i).1 = (pSpec' (Fin.cast round_eq i)).1
+  typeEquiv : ∀ i, (pSpec i).2 ≃ (pSpec' (Fin.cast round_eq i)).2
+
+namespace Equiv
+
+-- Note: this is not quite an `EquivLike` since `pSpec`s are terms, not types
+
+variable {m n k : ℕ} {pSpec : ProtocolSpec m} {pSpec' : ProtocolSpec n} {pSpec'' : ProtocolSpec k}
+
+@[simps]
+def refl (pSpec : ProtocolSpec n) : Equiv pSpec pSpec where
+  round_eq := rfl
+  dir_eq := fun _ => rfl
+  typeEquiv := fun _ => _root_.Equiv.refl _
+
+def symm (eqv : Equiv pSpec pSpec') : Equiv pSpec' pSpec where
+  round_eq := eqv.round_eq.symm
+  dir_eq := fun i => by simp [eqv.dir_eq]
+  typeEquiv := fun i => (eqv.typeEquiv (Fin.cast (eqv.round_eq.symm) i)).symm
+
+def trans (eqv : Equiv pSpec pSpec') (eqv' : Equiv pSpec' pSpec'') : Equiv pSpec pSpec'' where
+  round_eq := eqv.round_eq.trans eqv'.round_eq
+  dir_eq := fun i => by simp [eqv.dir_eq, eqv'.dir_eq]
+  typeEquiv := fun i => .trans (eqv.typeEquiv i) (eqv'.typeEquiv (Fin.cast eqv.round_eq i))
+
+end Equiv
+
+
+end ProtocolSpec
+
+/- Lots of TODOs here:
+
+1. Specify equivalence of transcripts, provers, verifiers, reductions
+2. Prove distributional equivalence of execution semantics
+3. Prove preservation of security properties
+-/
 
 variable {n : ℕ} {pSpec pSpec' : ProtocolSpec n}
 
 -- More targeted / limited version of equivalence only for the context, i.e.
 -- `ctxEquiv`, `stmtEquiv`, `oStmtEquiv`, `witEquiv`
 
--- Also, equality and not just equivalence. many times we want observational **equality**. have to specify fewer things
+-- Also, equality and not just equivalence. many times we want observational **equality**. have to
+-- specify fewer things
 
 -- Finally, could we go for a general _simulation_ relation?
 
-structure Prover.ObsEquiv (P : Prover pSpec oSpec StmtIn WitIn StmtOut WitOut)
-    (P' : Prover pSpec' oSpec' StmtIn' WitIn' StmtOut' WitOut') where
-  pSpecDirEq : ∀ i, (pSpec i).1 = (pSpec' i).1
-  pSpecEquiv : ∀ i, (pSpec i).2 ≃ (pSpec' i).2
-  stmtInEquiv : StmtIn ≃ StmtIn'
-  witInEquiv : WitIn ≃ WitIn'
-  stmtOutEquiv : StmtOut ≃ StmtOut'
-  witOutEquiv : WitOut ≃ WitOut'
+-- structure Prover.ObsEquiv (P : Prover pSpec oSpec StmtIn WitIn StmtOut WitOut)
+--     (P' : Prover pSpec' oSpec' StmtIn' WitIn' StmtOut' WitOut') where
+--   pSpecDirEq : ∀ i, (pSpec i).1 = (pSpec' i).1
+--   pSpecEquiv : ∀ i, (pSpec i).2 ≃ (pSpec' i).2
+--   stmtInEquiv : StmtIn ≃ StmtIn'
+--   witInEquiv : WitIn ≃ WitIn'
+--   stmtOutEquiv : StmtOut ≃ StmtOut'
+--   witOutEquiv : WitOut ≃ WitOut'
   -- All prover functions give the same output
   -- proverEquiv : ∀ stmtIn witIn, ...
 
